[llir-semantics] Evaluation rules for stores and syscalls.

test/syscall.c
@@ -1,0 +1,11 @@
+
+static __inline long __syscall0(long n)
+{
+  unsigned long ret;
+  __asm__ __volatile__ ("syscall" : "=a"(ret) : "a"(n) : "rcx", "r11", "memory");
+  return ret;
+}
+
+int main() {
+  return __syscall0(1000);
+}
