Syscall.v
@@ -1,0 +1,803 @@
+(* This file is part of the LLIR Semantics project. *)
+(* Licensing information is available in the LICENSE file. *)
+(* (C) 2020 Nandor Licker. All rights reserved. *)
+
+Require Import Coq.Bool.Bool.
+Require Import Coq.Lists.List.
+
+Require Import LLIR.Values.
+Require Import LLIR.Eval.
+Require Import LLIR.Maps.
+Require Import LLIR.Signal.
+Require Import LLIR.Types.
+
+Import ListNotations.
+
+Axiom ENOSYS: INT.I64.t.
+
+Inductive syscall :=
+  | sys_read
+  | sys_write
+  | sys_open
+  | sys_close
+  | sys_stat
+  | sys_fstat
+  | sys_lstat
+  | sys_poll
+  | sys_lseek
+  | sys_mmap
+  | sys_mprotect
+  | sys_munmap
+  | sys_brk
+  | sys_rt_sigaction
+  | sys_rt_sigprocmask
+  | sys_rt_sigreturn
+  | sys_ioctl
+  | sys_pread64
+  | sys_pwrite64
+  | sys_readv
+  | sys_writev
+  | sys_access
+  | sys_pipe
+  | sys_select
+  | sys_sched_yield
+  | sys_mremap
+  | sys_msync
+  | sys_mincore
+  | sys_madvise
+  | sys_shmget
+  | sys_shmat
+  | sys_shmctl
+  | sys_dup
+  | sys_dup2
+  | sys_pause
+  | sys_nanosleep
+  | sys_getitimer
+  | sys_alarm
+  | sys_setitimer
+  | sys_getpid
+  | sys_sendfile
+  | sys_socket
+  | sys_connect
+  | sys_accept
+  | sys_sendto
+  | sys_recvfrom
+  | sys_sendmsg
+  | sys_recvmsg
+  | sys_shutdown
+  | sys_bind
+  | sys_listen
+  | sys_getsockname
+  | sys_getpeername
+  | sys_socketpair
+  | sys_setsockopt
+  | sys_getsockopt
+  | sys_clone
+  | sys_fork
+  | sys_vfork
+  | sys_execve
+  | sys_exit
+  | sys_wait4
+  | sys_kill
+  | sys_uname
+  | sys_semget
+  | sys_semop
+  | sys_semctl
+  | sys_shmdt
+  | sys_msgget
+  | sys_msgsnd
+  | sys_msgrcv
+  | sys_msgctl
+  | sys_fcntl
+  | sys_flock
+  | sys_fsync
+  | sys_fdatasync
+  | sys_truncate
+  | sys_ftruncate
+  | sys_getdents
+  | sys_getcwd
+  | sys_chdir
+  | sys_fchdir
+  | sys_rename
+  | sys_mkdir
+  | sys_rmdir
+  | sys_creat
+  | sys_link
+  | sys_unlink
+  | sys_symlink
+  | sys_readlink
+  | sys_chmod
+  | sys_fchmod
+  | sys_chown
+  | sys_fchown
+  | sys_lchown
+  | sys_umask
+  | sys_gettimeofday
+  | sys_getrlimit
+  | sys_getrusage
+  | sys_sysinfo
+  | sys_times
+  | sys_ptrace
+  | sys_getuid
+  | sys_syslog
+  | sys_getgid
+  | sys_setuid
+  | sys_setgid
+  | sys_geteuid
+  | sys_getegid
+  | sys_setpgid
+  | sys_getppid
+  | sys_getpgrp
+  | sys_setsid
+  | sys_setreuid
+  | sys_setregid
+  | sys_getgroups
+  | sys_setgroups
+  | sys_setresuid
+  | sys_getresuid
+  | sys_setresgid
+  | sys_getresgid
+  | sys_getpgid
+  | sys_setfsuid
+  | sys_setfsgid
+  | sys_getsid
+  | sys_capget
+  | sys_capset
+  | sys_rt_sigpending
+  | sys_rt_sigtimedwait
+  | sys_rt_sigqueueinfo
+  | sys_rt_sigsuspend
+  | sys_sigaltstack
+  | sys_utime
+  | sys_mknod
+  | sys_uselib
+  | sys_personality
+  | sys_ustat
+  | sys_statfs
+  | sys_fstatfs
+  | sys_sysfs
+  | sys_getpriority
+  | sys_setpriority
+  | sys_sched_setparam
+  | sys_sched_getparam
+  | sys_sched_setscheduler
+  | sys_sched_getscheduler
+  | sys_sched_get_priority_max
+  | sys_sched_get_priority_min
+  | sys_sched_rr_get_interval
+  | sys_mlock
+  | sys_munlock
+  | sys_mlockall
+  | sys_munlockall
+  | sys_vhangup
+  | sys_modify_ldt
+  | sys_pivot_root
+  | sys__sysctl
+  | sys_prctl
+  | sys_arch_prctl
+  | sys_adjtimex
+  | sys_setrlimit
+  | sys_chroot
+  | sys_sync
+  | sys_acct
+  | sys_settimeofday
+  | sys_mount
+  | sys_umount2
+  | sys_swapon
+  | sys_swapoff
+  | sys_reboot
+  | sys_sethostname
+  | sys_setdomainname
+  | sys_iopl
+  | sys_ioperm
+  | sys_create_module
+  | sys_init_module
+  | sys_delete_module
+  | sys_get_kernel_syms
+  | sys_query_module
+  | sys_quotactl
+  | sys_nfsservctl
+  | sys_getpmsg
+  | sys_putpmsg
+  | sys_afs_syscall
+  | sys_tuxcall
+  | sys_security
+  | sys_gettid
+  | sys_readahead
+  | sys_setxattr
+  | sys_lsetxattr
+  | sys_fsetxattr
+  | sys_getxattr
+  | sys_lgetxattr
+  | sys_fgetxattr
+  | sys_listxattr
+  | sys_llistxattr
+  | sys_flistxattr
+  | sys_removexattr
+  | sys_lremovexattr
+  | sys_fremovexattr
+  | sys_tkill
+  | sys_time
+  | sys_futex
+  | sys_sched_setaffinity
+  | sys_sched_getaffinity
+  | sys_set_thread_area
+  | sys_io_setup
+  | sys_io_destroy
+  | sys_io_getevents
+  | sys_io_submit
+  | sys_io_cancel
+  | sys_get_thread_area
+  | sys_lookup_dcookie
+  | sys_epoll_create
+  | sys_epoll_ctl_old
+  | sys_epoll_wait_old
+  | sys_remap_file_pages
+  | sys_getdents64
+  | sys_set_tid_address
+  | sys_restart_syscall
+  | sys_semtimedop
+  | sys_fadvise64
+  | sys_timer_create
+  | sys_timer_settime
+  | sys_timer_gettime
+  | sys_timer_getoverrun
+  | sys_timer_delete
+  | sys_clock_settime
+  | sys_clock_gettime
+  | sys_clock_getres
+  | sys_clock_nanosleep
+  | sys_exit_group
+  | sys_epoll_wait
+  | sys_epoll_ctl
+  | sys_tgkill
+  | sys_utimes
+  | sys_vserver
+  | sys_mbind
+  | sys_set_mempolicy
+  | sys_get_mempolicy
+  | sys_mq_open
+  | sys_mq_unlink
+  | sys_mq_timedsend
+  | sys_mq_timedreceive
+  | sys_mq_notify
+  | sys_mq_getsetattr
+  | sys_kexec_load
+  | sys_waitid
+  | sys_add_key
+  | sys_request_key
+  | sys_keyctl
+  | sys_ioprio_set
+  | sys_ioprio_get
+  | sys_inotify_init
+  | sys_inotify_add_watch
+  | sys_inotify_rm_watch
+  | sys_migrate_pages
+  | sys_openat
+  | sys_mkdirat
+  | sys_mknodat
+  | sys_fchownat
+  | sys_futimesat
+  | sys_newfstatat
+  | sys_unlinkat
+  | sys_renameat
+  | sys_linkat
+  | sys_symlinkat
+  | sys_readlinkat
+  | sys_fchmodat
+  | sys_faccessat
+  | sys_pselect6
+  | sys_ppoll
+  | sys_unshare
+  | sys_set_robust_list
+  | sys_get_robust_list
+  | sys_splice
+  | sys_tee
+  | sys_sync_file_range
+  | sys_vmsplice
+  | sys_move_pages
+  | sys_utimensat
+  | sys_epoll_pwait
+  | sys_signalfd
+  | sys_timerfd_create
+  | sys_eventfd
+  | sys_fallocate
+  | sys_timerfd_settime
+  | sys_timerfd_gettime
+  | sys_accept4
+  | sys_signalfd4
+  | sys_eventfd2
+  | sys_epoll_create1
+  | sys_dup3
+  | sys_pipe2
+  | sys_inotify_init1
+  | sys_preadv
+  | sys_pwritev
+  | sys_rt_tgsigqueueinfo
+  | sys_perf_event_open
+  | sys_recvmmsg
+  | sys_fanotify_init
+  | sys_fanotify_mark
+  | sys_prlimit64
+  | sys_name_to_handle_at
+  | sys_open_by_handle_at
+  | sys_clock_adjtime
+  | sys_syncfs
+  | sys_sendmmsg
+  | sys_setns
+  | sys_getcpu
+  | sys_process_vm_readv
+  | sys_process_vm_writev
+  | sys_kcmp
+  | sys_finit_module
+  | sys_sched_setattr
+  | sys_sched_getattr
+  | sys_renameat2
+  | sys_seccomp
+  | sys_getrandom
+  | sys_memfd_create
+  | sys_kexec_file_load
+  | sys_bpf
+  | sys_execveat
+  | sys_userfaultfd
+  | sys_membarrier
+  | sys_mlock2
+  | sys_copy_file_range
+  | sys_preadv2
+  | sys_pwritev2
+  | sys_pkey_mprotect
+  | sys_pkey_alloc
+  | sys_pkey_free
+  | sys_statx
+  | sys_io_pgetevents
+  | sys_rseq
+  | sys_pidfd_send_signal
+  | sys_io_uring_setup
+  | sys_io_uring_enter
+  | sys_io_uring_register
+  | sys_open_tree
+  | sys_move_mount
+  | sys_fsopen
+  | sys_fsconfig
+  | sys_fsmount
+  | sys_fspick
+  .
+
+Definition syscall_of_sno (sno: INT.I64.t): option syscall :=
+  match INT.I64.to_nat sno with
+  |   0 => Some sys_read
+  |   1 => Some sys_write
+  |   2 => Some sys_open
+  |   3 => Some sys_close
+  |   4 => Some sys_stat
+  |   5 => Some sys_fstat
+  |   6 => Some sys_lstat
+  |   7 => Some sys_poll
+  |   8 => Some sys_lseek
+  |   9 => Some sys_mmap
+  |  10 => Some sys_mprotect
+  |  11 => Some sys_munmap
+  |  12 => Some sys_brk
+  |  13 => Some sys_rt_sigaction
+  |  14 => Some sys_rt_sigprocmask
+  |  15 => Some sys_rt_sigreturn
+  |  16 => Some sys_ioctl
+  |  17 => Some sys_pread64
+  |  18 => Some sys_pwrite64
+  |  19 => Some sys_readv
+  |  20 => Some sys_writev
+  |  21 => Some sys_access
+  |  22 => Some sys_pipe
+  |  23 => Some sys_select
+  |  24 => Some sys_sched_yield
+  |  25 => Some sys_mremap
+  |  26 => Some sys_msync
+  |  27 => Some sys_mincore
+  |  28 => Some sys_madvise
+  |  29 => Some sys_shmget
+  |  30 => Some sys_shmat
+  |  31 => Some sys_shmctl
+  |  32 => Some sys_dup
+  |  33 => Some sys_dup2
+  |  34 => Some sys_pause
+  |  35 => Some sys_nanosleep
+  |  36 => Some sys_getitimer
+  |  37 => Some sys_alarm
+  |  38 => Some sys_setitimer
+  |  39 => Some sys_getpid
+  |  40 => Some sys_sendfile
+  |  41 => Some sys_socket
+  |  42 => Some sys_connect
+  |  43 => Some sys_accept
+  |  44 => Some sys_sendto
+  |  45 => Some sys_recvfrom
+  |  46 => Some sys_sendmsg
+  |  47 => Some sys_recvmsg
+  |  48 => Some sys_shutdown
+  |  49 => Some sys_bind
+  |  50 => Some sys_listen
+  |  51 => Some sys_getsockname
+  |  52 => Some sys_getpeername
+  |  53 => Some sys_socketpair
+  |  54 => Some sys_setsockopt
+  |  55 => Some sys_getsockopt
+  |  56 => Some sys_clone
+  |  57 => Some sys_fork
+  |  58 => Some sys_vfork
+  |  59 => Some sys_execve
+  |  60 => Some sys_exit
+  |  61 => Some sys_wait4
+  |  62 => Some sys_kill
+  |  63 => Some sys_uname
+  |  64 => Some sys_semget
+  |  65 => Some sys_semop
+  |  66 => Some sys_semctl
+  |  67 => Some sys_shmdt
+  |  68 => Some sys_msgget
+  |  69 => Some sys_msgsnd
+  |  70 => Some sys_msgrcv
+  |  71 => Some sys_msgctl
+  |  72 => Some sys_fcntl
+  |  73 => Some sys_flock
+  |  74 => Some sys_fsync
+  |  75 => Some sys_fdatasync
+  |  76 => Some sys_truncate
+  |  77 => Some sys_ftruncate
+  |  78 => Some sys_getdents
+  |  79 => Some sys_getcwd
+  |  80 => Some sys_chdir
+  |  81 => Some sys_fchdir
+  |  82 => Some sys_rename
+  |  83 => Some sys_mkdir
+  |  84 => Some sys_rmdir
+  |  85 => Some sys_creat
+  |  86 => Some sys_link
+  |  87 => Some sys_unlink
+  |  88 => Some sys_symlink
+  |  89 => Some sys_readlink
+  |  90 => Some sys_chmod
+  |  91 => Some sys_fchmod
+  |  92 => Some sys_chown
+  |  93 => Some sys_fchown
+  |  94 => Some sys_lchown
+  |  95 => Some sys_umask
+  |  96 => Some sys_gettimeofday
+  |  97 => Some sys_getrlimit
+  |  98 => Some sys_getrusage
+  |  99 => Some sys_sysinfo
+  | 100 => Some sys_times
+  | 101 => Some sys_ptrace
+  | 102 => Some sys_getuid
+  | 103 => Some sys_syslog
+  | 104 => Some sys_getgid
+  | 105 => Some sys_setuid
+  | 106 => Some sys_setgid
+  | 107 => Some sys_geteuid
+  | 108 => Some sys_getegid
+  | 109 => Some sys_setpgid
+  | 110 => Some sys_getppid
+  | 111 => Some sys_getpgrp
+  | 112 => Some sys_setsid
+  | 113 => Some sys_setreuid
+  | 114 => Some sys_setregid
+  | 115 => Some sys_getgroups
+  | 116 => Some sys_setgroups
+  | 117 => Some sys_setresuid
+  | 118 => Some sys_getresuid
+  | 119 => Some sys_setresgid
+  | 120 => Some sys_getresgid
+  | 121 => Some sys_getpgid
+  | 122 => Some sys_setfsuid
+  | 123 => Some sys_setfsgid
+  | 124 => Some sys_getsid
+  | 125 => Some sys_capget
+  | 126 => Some sys_capset
+  | 127 => Some sys_rt_sigpending
+  | 128 => Some sys_rt_sigtimedwait
+  | 129 => Some sys_rt_sigqueueinfo
+  | 130 => Some sys_rt_sigsuspend
+  | 131 => Some sys_sigaltstack
+  | 132 => Some sys_utime
+  | 133 => Some sys_mknod
+  | 134 => Some sys_uselib
+  | 135 => Some sys_personality
+  | 136 => Some sys_ustat
+  | 137 => Some sys_statfs
+  | 138 => Some sys_fstatfs
+  | 139 => Some sys_sysfs
+  | 140 => Some sys_getpriority
+  | 141 => Some sys_setpriority
+  | 142 => Some sys_sched_setparam
+  | 143 => Some sys_sched_getparam
+  | 144 => Some sys_sched_setscheduler
+  | 145 => Some sys_sched_getscheduler
+  | 146 => Some sys_sched_get_priority_max
+  | 147 => Some sys_sched_get_priority_min
+  | 148 => Some sys_sched_rr_get_interval
+  | 149 => Some sys_mlock
+  | 150 => Some sys_munlock
+  | 151 => Some sys_mlockall
+  | 152 => Some sys_munlockall
+  | 153 => Some sys_vhangup
+  | 154 => Some sys_modify_ldt
+  | 155 => Some sys_pivot_root
+  | 156 => Some sys__sysctl
+  | 157 => Some sys_prctl
+  | 158 => Some sys_arch_prctl
+  | 159 => Some sys_adjtimex
+  | 160 => Some sys_setrlimit
+  | 161 => Some sys_chroot
+  | 162 => Some sys_sync
+  | 163 => Some sys_acct
+  | 164 => Some sys_settimeofday
+  | 165 => Some sys_mount
+  | 166 => Some sys_umount2
+  | 167 => Some sys_swapon
+  | 168 => Some sys_swapoff
+  | 169 => Some sys_reboot
+  | 170 => Some sys_sethostname
+  | 171 => Some sys_setdomainname
+  | 172 => Some sys_iopl
+  | 173 => Some sys_ioperm
+  | 174 => Some sys_create_module
+  | 175 => Some sys_init_module
+  | 176 => Some sys_delete_module
+  | 177 => Some sys_get_kernel_syms
+  | 178 => Some sys_query_module
+  | 179 => Some sys_quotactl
+  | 180 => Some sys_nfsservctl
+  | 181 => Some sys_getpmsg
+  | 182 => Some sys_putpmsg
+  | 183 => Some sys_afs_syscall
+  | 184 => Some sys_tuxcall
+  | 185 => Some sys_security
+  | 186 => Some sys_gettid
+  | 187 => Some sys_readahead
+  | 188 => Some sys_setxattr
+  | 189 => Some sys_lsetxattr
+  | 190 => Some sys_fsetxattr
+  | 191 => Some sys_getxattr
+  | 192 => Some sys_lgetxattr
+  | 193 => Some sys_fgetxattr
+  | 194 => Some sys_listxattr
+  | 195 => Some sys_llistxattr
+  | 196 => Some sys_flistxattr
+  | 197 => Some sys_removexattr
+  | 198 => Some sys_lremovexattr
+  | 199 => Some sys_fremovexattr
+  | 200 => Some sys_tkill
+  | 201 => Some sys_time
+  | 202 => Some sys_futex
+  | 203 => Some sys_sched_setaffinity
+  | 204 => Some sys_sched_getaffinity
+  | 205 => Some sys_set_thread_area
+  | 206 => Some sys_io_setup
+  | 207 => Some sys_io_destroy
+  | 208 => Some sys_io_getevents
+  | 209 => Some sys_io_submit
+  | 210 => Some sys_io_cancel
+  | 211 => Some sys_get_thread_area
+  | 212 => Some sys_lookup_dcookie
+  | 213 => Some sys_epoll_create
+  | 214 => Some sys_epoll_ctl_old
+  | 215 => Some sys_epoll_wait_old
+  | 216 => Some sys_remap_file_pages
+  | 217 => Some sys_getdents64
+  | 218 => Some sys_set_tid_address
+  | 219 => Some sys_restart_syscall
+  | 220 => Some sys_semtimedop
+  | 221 => Some sys_fadvise64
+  | 222 => Some sys_timer_create
+  | 223 => Some sys_timer_settime
+  | 224 => Some sys_timer_gettime
+  | 225 => Some sys_timer_getoverrun
+  | 226 => Some sys_timer_delete
+  | 227 => Some sys_clock_settime
+  | 228 => Some sys_clock_gettime
+  | 229 => Some sys_clock_getres
+  | 230 => Some sys_clock_nanosleep
+  | 231 => Some sys_exit_group
+  | 232 => Some sys_epoll_wait
+  | 233 => Some sys_epoll_ctl
+  | 234 => Some sys_tgkill
+  | 235 => Some sys_utimes
+  | 236 => Some sys_vserver
+  | 237 => Some sys_mbind
+  | 238 => Some sys_set_mempolicy
+  | 239 => Some sys_get_mempolicy
+  | 240 => Some sys_mq_open
+  | 241 => Some sys_mq_unlink
+  | 242 => Some sys_mq_timedsend
+  | 243 => Some sys_mq_timedreceive
+  | 244 => Some sys_mq_notify
+  | 245 => Some sys_mq_getsetattr
+  | 246 => Some sys_kexec_load
+  | 247 => Some sys_waitid
+  | 248 => Some sys_add_key
+  | 249 => Some sys_request_key
+  | 250 => Some sys_keyctl
+  | 251 => Some sys_ioprio_set
+  | 252 => Some sys_ioprio_get
+  | 253 => Some sys_inotify_init
+  | 254 => Some sys_inotify_add_watch
+  | 255 => Some sys_inotify_rm_watch
+  | 256 => Some sys_migrate_pages
+  | 257 => Some sys_openat
+  | 258 => Some sys_mkdirat
+  | 259 => Some sys_mknodat
+  | 260 => Some sys_fchownat
+  | 261 => Some sys_futimesat
+  | 262 => Some sys_newfstatat
+  | 263 => Some sys_unlinkat
+  | 264 => Some sys_renameat
+  | 265 => Some sys_linkat
+  | 266 => Some sys_symlinkat
+  | 267 => Some sys_readlinkat
+  | 268 => Some sys_fchmodat
+  | 269 => Some sys_faccessat
+  | 270 => Some sys_pselect6
+  | 271 => Some sys_ppoll
+  | 272 => Some sys_unshare
+  | 273 => Some sys_set_robust_list
+  | 274 => Some sys_get_robust_list
+  | 275 => Some sys_splice
+  | 276 => Some sys_tee
+  | 277 => Some sys_sync_file_range
+  | 278 => Some sys_vmsplice
+  | 279 => Some sys_move_pages
+  | 280 => Some sys_utimensat
+  | 281 => Some sys_epoll_pwait
+  | 282 => Some sys_signalfd
+  | 283 => Some sys_timerfd_create
+  | 284 => Some sys_eventfd
+  | 285 => Some sys_fallocate
+  | 286 => Some sys_timerfd_settime
+  | 287 => Some sys_timerfd_gettime
+  | 288 => Some sys_accept4
+  | 289 => Some sys_signalfd4
+  | 290 => Some sys_eventfd2
+  | 291 => Some sys_epoll_create1
+  | 292 => Some sys_dup3
+  | 293 => Some sys_pipe2
+  | 294 => Some sys_inotify_init1
+  | 295 => Some sys_preadv
+  | 296 => Some sys_pwritev
+  | 297 => Some sys_rt_tgsigqueueinfo
+  | 298 => Some sys_perf_event_open
+  | 299 => Some sys_recvmmsg
+  | 300 => Some sys_fanotify_init
+  | 301 => Some sys_fanotify_mark
+  | 302 => Some sys_prlimit64
+  | 303 => Some sys_name_to_handle_at
+  | 304 => Some sys_open_by_handle_at
+  | 305 => Some sys_clock_adjtime
+  | 306 => Some sys_syncfs
+  | 307 => Some sys_sendmmsg
+  | 308 => Some sys_setns
+  | 309 => Some sys_getcpu
+  | 310 => Some sys_process_vm_readv
+  | 311 => Some sys_process_vm_writev
+  | 312 => Some sys_kcmp
+  | 313 => Some sys_finit_module
+  | 314 => Some sys_sched_setattr
+  | 315 => Some sys_sched_getattr
+  | 316 => Some sys_renameat2
+  | 317 => Some sys_seccomp
+  | 318 => Some sys_getrandom
+  | 319 => Some sys_memfd_create
+  | 320 => Some sys_kexec_file_load
+  | 321 => Some sys_bpf
+  | 322 => Some sys_execveat
+  | 323 => Some sys_userfaultfd
+  | 324 => Some sys_membarrier
+  | 325 => Some sys_mlock2
+  | 326 => Some sys_copy_file_range
+  | 327 => Some sys_preadv2
+  | 328 => Some sys_pwritev2
+  | 329 => Some sys_pkey_mprotect
+  | 330 => Some sys_pkey_alloc
+  | 331 => Some sys_pkey_free
+  | 332 => Some sys_statx
+  | 333 => Some sys_io_pgetevents
+  | 334 => Some sys_rseq
+  | 424 => Some sys_pidfd_send_signal
+  | 425 => Some sys_io_uring_setup
+  | 426 => Some sys_io_uring_enter
+  | 427 => Some sys_io_uring_register
+  | 428 => Some sys_open_tree
+  | 429 => Some sys_move_mount
+  | 430 => Some sys_fsopen
+  | 431 => Some sys_fsconfig
+  | 432 => Some sys_fsmount
+  | 433 => Some sys_fspick
+  | _ => None
+  end.
+
+
+Inductive SyscallNumber : value -> syscall -> Prop :=
+  | syscall_sys:
+    forall (v: INT.I64.t) (s: syscall) (SNO_CALL: Some s = syscall_of_sno v),
+      SyscallNumber (VInt (INT.Int64 v)) s
+  .
+
+Inductive SyscallNoSys : value -> Prop :=
+  | syscall_no_sys:
+    forall (v: INT.I64.t) (SNO_CALL: None = syscall_of_sno v),
+      SyscallNoSys (VInt (INT.Int64 v))
+  .
+
+Inductive SyscallUndef : value -> Prop :=
+  | syscall_undef_sym: forall (s: sym), SyscallUndef (VSym s)
+  | syscall_undef_und: SyscallUndef VUnd
+  .
+
+Lemma syscall_number_complete:
+  forall (v: value),
+    TypeOfValue v (TInt I64) ->
+    (exists (s: syscall), SyscallNumber v s)
+    \/
+    SyscallNoSys v
+    \/
+    SyscallUndef v.
+Proof.
+  intros v Hty. inversion Hty; subst.
+  - inversion TY; subst.
+    destruct (syscall_of_sno v) as [s|] eqn:Esno.
+    + left; exists s; constructor; auto.
+    + right; left; constructor; auto.
+  - right; right; constructor.
+  - right; right; constructor.
+Qed.
+
+Inductive SyscallArg : reg -> value -> Prop :=
+  | sys_arg_und: forall (r: reg), SyscallArg r VUnd
+  | sys_arg_sym: forall (r: reg) (s: sym), SyscallArg r (VSym s)
+  | sys_arg_int: forall (r: reg) (i: INT.I64.t), SyscallArg r (VInt (INT.Int64 i))
+  .
+
+Inductive SyscallArgs : frame -> list reg -> list value -> Prop :=
+  | arg_vals_nil:
+    forall
+      (fr: frame),
+      SyscallArgs fr [] []
+  | arg_vals_cons:
+    forall
+      (fr: frame)
+      (arg_value: value) (arg_values: list value)
+      (arg: reg) (args: list reg)
+      (VALUE: Some arg_value = fr.(fr_regs) ! arg)
+      (HEAD: SyscallArg arg arg_value)
+      (TAIL: SyscallArgs fr args arg_values),
+      SyscallArgs fr (arg::args) (arg_value::arg_values)
+  .
+
+Inductive SyscallRet 
+  : syscall ->
+    list value ->
+    stack -> 
+    heap -> 
+    trace -> 
+    stack -> 
+    heap -> 
+    INT.I64.t -> 
+    Prop :=
+  .
+
+Inductive SyscallSig 
+  : syscall ->
+    list value ->
+    stack -> 
+    heap -> 
+    trace -> 
+    signal -> 
+    Prop :=
+  .
+
+Lemma syscall_ret_or_sig :
+  forall (sno: syscall) (args: list value) (stk: stack) (h: heap),
+    {exists (tr: trace) (stk': stack) (h': heap) (v: INT.I64.t), 
+      SyscallRet sno args stk h tr stk' h' v}
+    +
+    {exists (sig: signal) (tr: trace), 
+      SyscallSig sno args stk h tr sig}.
+Admitted.
